

Some Interesting Problems

Saptarshi Dey

20 February, 2021

1 Equations with Complex Solutions

$$\begin{aligned}\sin(x)^{\sin(x)} &= 2 \\ \implies \sin(x) \ln(\sin(x)) &= \ln(2)\end{aligned}$$

Let's assume $\sin(x) = e^a$

$$\begin{aligned}\therefore ae^a &= \ln(2) \\ \implies a &= W(\ln(2))\end{aligned}$$

W is the Lambert W function

$$\begin{aligned}\therefore \sin(x) &= e^{W(\ln(2))} \\ \sin(x) &= e^{W(0.6931)} = 1.5596 \approx 1.56\end{aligned}$$

Clearly this has no real solution. But there might be a complex one:

$$\sin(x) = \frac{e^{ix} - e^{-ix}}{2i} = 1.56$$

Let's assume $u = e^{ix}$

$$\begin{aligned}\therefore u - u^{-1} &= 3.12i \\ \implies u^2 - 3.12iu - 1 &= 0\end{aligned}$$

Taking $a = 1, b = -3.12i, c = -1$

$$\begin{aligned}\therefore u &= \frac{3.12i \pm \sqrt{-9.7344 + 4}}{2} \\ \therefore u &= \frac{3.12i \pm 2.4i}{2} = 1.56i \pm 1.2i \\ \therefore e^{ix} &= 1.56i \pm 1.2i \\ ix &= \ln(1.56i \pm 1.2i) = \ln(i) + \ln(1.56 \pm 1.2)\end{aligned}$$

We know, $i = e^{i\pi/2}$

$$\begin{aligned}\therefore ix &= \frac{\pi}{2}i + \ln(1.56 \pm 1.2) \\ \implies \boxed{x = \frac{\pi}{2} - \ln(1.56 \pm 1.2)i}\end{aligned}$$

2 Feynman's Technique of Integration

2.1 Evaluate the following using Feynman's Technique

1. $\int_0^\infty e^{-x^2} \cos(5x) dx$
2. $\int_0^1 \frac{\sin(\ln(x))}{\ln(x)} dx$

2.2 Solution

$$1. \text{ Let } I(\alpha) = \int_0^{\infty} e^{-x^2} \cos(\alpha x) dx$$

$$\Rightarrow I'(\alpha) = \int_0^{\infty} \frac{\delta}{\delta \alpha} \left(e^{-x^2} \cos(\alpha x) \right) dx = - \int_0^{\infty} x e^{-x^2} \sin(\alpha x) dx$$

Integrating by parts

$$I'(\alpha) = \left[\frac{\sin(\alpha x)}{2e^{x^2}} \right]_0^{\infty} - \frac{\alpha}{2} \int_0^{\infty} e^{-x^2} \cos(\alpha x) dx \Rightarrow I'(\alpha) = 0 - \frac{\alpha}{2} I(\alpha)$$

$$\therefore \int \frac{d[I(\alpha)]}{I(\alpha)} = \frac{-1}{2} \int \alpha d\alpha \Rightarrow \ln(I(\alpha)) = \frac{-\alpha^2}{4} + C' \Rightarrow I(\alpha) = C e^{-\alpha^2/4}$$

$$\text{We know that } I(0) = \int_0^{\infty} e^{-x^2} dx = \frac{\sqrt{\pi}}{2} \text{ (The Gaussian Integral)}$$

$$\therefore C = \frac{\sqrt{\pi}}{2} \therefore I(\alpha) = \frac{\sqrt{\pi}}{2} e^{-\alpha^2/4} \text{ and } I(5) = \boxed{\frac{\sqrt{\pi}}{2} e^{-25/4}}$$

2. Using the complex form of the sin function we get

$$\int_0^1 \frac{\sin(\ln(x))}{\ln(x)} dx = \int_0^1 \frac{x^i - x^{-i}}{2i \ln(x)} dx$$

$$\text{Let } I(b) = \int_0^1 \frac{x^{bi} - x^{-i}}{2i \ln(x)} dx$$

$$\therefore I'(b) = \int_0^1 \frac{\delta}{\delta b} \left(\frac{x^{bi} - x^{-i}}{2i \ln(x)} \right) dx = \int_0^1 \frac{x^{bi} i \ln(x)}{2i \ln(x)} dx = \frac{1}{2(1+bi)} [x^{1+bi}]_0^1 = \frac{1}{2(1+bi)}$$

$$\therefore I(b) = \frac{1}{2} \int \frac{db}{1+bi} = \frac{1}{2i} \ln(1+bi) + C$$

Let $b = -1$

$$\therefore I(-1) = \int_0^1 \frac{x^{-i} - x^{-i}}{2i \ln(x)} dx = 0$$

$$\therefore \frac{1}{2i} \ln(1-i) + C = 0 \Rightarrow C = -\frac{1}{2i} \ln(1-i)$$

$$\therefore I(b) = \frac{\ln(1+bi) - \ln(1-i)}{2i} = \frac{1}{2i} \ln \left(\frac{1+bi}{1-i} \right)$$

$$\therefore I(1) = \frac{1}{2i} \ln \left(\frac{1+i}{1-i} \right) = \frac{1}{2i} \ln(e^{i\pi/2}) = \boxed{\frac{\pi}{4}}$$